cava/Cava/Acorn/Sequential.v
@@ -98,6 +98,13 @@ Definition loopSeq {A B C : SignalType}
   '(b, _) <- snd (fold_left (loopSeq' f) a (0, ret ([], [defaultCombValue C]))) ;;
   ret b.
 
+Definition loopSeqS {A B C : SignalType}
+                    (f : seqType A * seqType C -> ident (seqType B * seqType C))
+                    (a : seqType A) : ident (seqType B * seqType C) :=
+  snd (fold_left (loopSeq' f) a (0, ret ([], [defaultCombValue C]))).
+(* This is wrong, because I think it will return just the last element
+   for the current state output stream. *)
+
 (******************************************************************************)
 (* A boolean sequential logic interpretation for the Cava class               *)
 (******************************************************************************)
@@ -298,6 +305,7 @@ Definition delayEnableBoolList (t: SignalType) (en: list bool) (i : seqType t) :
    { delay t i := ret (@defaultCombValue t :: i);
      delayEnable t en i := delayEnableBoolList t en i; 
      loopDelay _ _ _ := loopSeq;
+     loopDelayS _ _ _ := loopSeqS;
      loopDelayEnable A B C en f :=
        (* The semantics of loopDelayEnable is defined in terms of loopDelay and
           the circuitry required to model a clock enable with a multiplexor. *)
@@ -307,6 +315,14 @@ Definition delayEnableBoolList (t: SignalType) (en: list bool) (i : seqType t) :
                     let '(en, i) := unpair (fst en_i_feedback) in
                     (second fork2 >=> pairLeft >=> first f >=> pairRight >=> second (swap >=> mux2 en))
                       (i, feedback)) (mkpair en i);
+     loopDelaySEnable A B C en f input :=
+       (* The semantics of loopDelaySEnable is defined in terms of loopDelayS and
+          the circuitry required to model a clock enable with a multiplexor. *)
+         loopSeqS (fun (en_i_feedback : seqType (Pair Bit A) * seqType C)  =>
+                     let feedback := snd en_i_feedback in
+                     let '(en, i) := unpair (fst en_i_feedback) in
+                     (second fork2 >=> pairLeft >=> first f >=> pairRight >=> second (swap >=> mux2 en))
+                       (i, feedback)) (mkpair en input)
    }.
 
 (******************************************************************************)
